theories/lang/cpp/logic/stmt.v
@@ -118,19 +118,19 @@ Module Type Stmt.
         let continue := local_addr ρ x a -* done in
         match init with
         | None =>
-          _at (_eqp a) (uninit (erase_qualifiers ty) 1) -* continue
+          _at (_eq a) (uninit (erase_qualifiers ty) 1) -* continue
         | Some init =>
           wp_prval init (fun v free => free **
-                              _at (_eqp a) (tprim (erase_qualifiers ty) 1 v) -* continue)
+                              _at (_eq a) (tprim (erase_qualifiers ty) 1 v) -* continue)
         end
 
       | Tref cls =>
-        Forall a, _at (_eqp a) (uninit (erase_qualifiers ty) 1) -*
+        Forall a, _at (_eq a) (uninit (erase_qualifiers ty) 1) -*
                   let destroy :=
                       match dtor with
                       | None => fun x => x
                       | Some dtor => destruct_obj ti dtor cls (Vptr a)
-                      end (_at (_eqp a) (tany (erase_qualifiers ty) 1))
+                      end (_at (_eq a) (tany (erase_qualifiers ty) 1))
                   in
                   let continue :=
                       local_addr ρ x a -* k (Kfree (local_addr ρ x a ** destroy) Q)
@@ -141,16 +141,16 @@ Module Type Stmt.
                     wp_init ty (Vptr a) (not_mine init) (fun free => free ** continue)
                   end
       | Tarray ty' N =>
-        Forall a, _at (_eqp a) (uninit (erase_qualifiers ty) 1) -*
+        Forall a, _at (_eq a) (uninit (erase_qualifiers ty) 1) -*
                   let destroy : mpred :=
                       match dtor with
                       | None => fun x => x
                       | Some dtor => destruct ti ty (Vptr a) dtor
-                      end (_at (_eqp a) (tany (erase_qualifiers ty) 1))
+                      end (_at (_eq a) (tany (erase_qualifiers ty) 1))
                   in
                   let continue :=
                       local_addr ρ x a -*
-                      k (Kfree (local_addr ρ x a ** _at (_eqp a) (tany (erase_qualifiers ty) 1)) Q)
+                      k (Kfree (local_addr ρ x a ** _at (_eq a) (tany (erase_qualifiers ty) 1)) Q)
                   in
                   match init with
                   | None => continue
